src/lemmas.lean
@@ -6,71 +6,291 @@ section
 
 set_option pp.structure_projections false
 
-open option
+local notation e ` ⟦` n ` ↦ ` e' `⟧`  := expr.subs e n e'
+local notation e ` ⟦` n ` ↟ ` m `⟧`   := expr.gap e n m
+local notation e ` ~> ` e'            := small e e'
+local notation e ` ~>* ` e'           := small_star e e'
+local notation Γ ` ⊢ ` e `: ` t       := has_type Γ e t
+local notation `⊢ ` Γ                 := ctx_wf Γ
+
+/- Auxiliary arithmetic lemmas. -/
+
+lemma nat.order_aux_1 {a b : nat} (h₁ : ¬a < b) (h₂ : ¬a = b) : (b < a) :=
+  ne.lt_of_le (ne.symm h₂) (le_of_not_gt h₁)
+
+lemma nat.order_aux_2 {a b c : nat} (h : a + b < c) : b < c :=
+  lt_of_le_of_lt (nat.le_add_left b a) h
+
+lemma nat.order_aux_3 {a b c : nat} (h : a + b < c) : a < c :=
+  lt_of_le_of_lt (nat.le_add_right a b) h
+
+lemma nat.le_add_left' (a b c : ℕ) (h : a ≤ b) : a ≤ c + b :=
+  le_add_left h
+
+lemma nat.le_add_right' (a b c : ℕ) (h : a ≤ b) : a ≤ b + c :=
+  le_add_right h
+
+-- #check @nat.le.intro
+-- #check @nat.le.dest
+
+namespace expr
+section
+
 open idx
-open expr
 
-local notation e `⟦` r `/$⟧`    := subs e 0 r
-local notation e ` ~> ` e'      := small e e'
-local notation e ` ~>* ` e'     := small_star e e'
-local notation Γ ` ⊢ ` e `: ` t := has_type Γ e t
-local notation `⊢ ` Γ           := ctx_wf Γ
+/- Uninteresting `gap` lemmas for supporting case analysis. -/
 
-namespace closed
+lemma gap_bound (v n m) : var (bound v) ⟦n ↟ m⟧ =
+  if n <= v then var (bound (v + m)) else var (bound v) := by unfold gap
 
-  /-- Lemmas for `closed e n`: `e` has at most `n` levels of unbound variables. -/
-  lemma c_sort (s n)                                                  : closed (sort s) n        := trivial
-  lemma c_bound {b n} (h : b < n)                                     : closed (var (bound b)) n := h
-  lemma c_free (f n)                                                  : closed (var (free f)) n  := trivial
-  lemma c_app {l r n} (hcl : closed l n) (hcr : closed r n)           : closed (app l r) n       := ⟨hcl, hcr⟩
-  lemma c_lam {t e n} (hct : closed t n) (hce : closed e n.succ)      : closed (lam t e) n       := ⟨hct, hce⟩
-  lemma c_pi {t₁ t₂ n} (hct₁ : closed t₁ n) (hct₂ : closed t₂ n.succ) : closed (pi t₁ t₂) n      := ⟨hct₁, hct₂⟩
+lemma gap_bound_n_le_v {v n m} (h : n ≤ v) :
+  var (bound v) ⟦n ↟ m⟧ = var (bound (v + m)) := by
+  { unfold gap, split_ifs, refl }
 
-  lemma c_weaken {e n n'} (hce : closed e n) (h : n <= n') : closed e n' :=
-    @expr.rec (λ e, ∀ n n', n ≤ n' → closed e n → closed e n')
-      (λ _ _ _ _ _, c_sort _ _)
-      (λ v _ _ h,
-        match v with
-        | (bound b) := λ hcb, c_bound (nat.lt_of_lt_of_le hcb h)
-        | (free f) := λ hcf, c_free _ _
-        end)
-      (λ _ _ hl hr _ _ h ⟨hcl, hcr⟩, ⟨hl _ _ h hcl, hr _ _ h hcr⟩)
-      (λ _ _ ht he _ _ h ⟨hct, hce⟩, ⟨ht _ _ h hct, he _ _ (nat.succ_le_succ h) hce⟩)
-      (λ _ _ ht₁ ht₂ _ _ h ⟨hct₁, hct₂⟩, ⟨ht₁ _ _ h hct₁, ht₂ _ _ (nat.succ_le_succ h) hct₂⟩)
-      e n n' h hce
+lemma gap_bound_v_lt_n {v n m} (h : v < n) :
+  var (bound v) ⟦n ↟ m⟧ = var (bound v) := by
+  { unfold gap, split_ifs with hif, exfalso, exact not_le_of_lt h hif, refl }
 
-  lemma c_weaken₁ {e n} (hce : closed e n) : closed e n.succ :=
-    c_weaken hce (nat.le_succ n)
+/- Uninteresting `subs` lemmas for supporting case analysis. -/
 
-end closed
-open closed
+lemma subs_bound (v n e') : var (bound v) ⟦n ↦ e'⟧ =
+  if n < v then var (bound v.pred)
+  else if n = v then e'.gap 0 n
+  else (var (bound v)) := by unfold subs
 
-/-- Substitution at the topmost level "closes" that level of unbound variables. -/
-lemma subs.close {e e'} {n : nat} :
-  closed e n.succ → closed e' n → closed (subs e n e') n := by
-{ intros hce hce',
-  induction e generalizing n,
+lemma subs_bound_n_lt_v {v n e'} (h : n < v) :
+  var (bound v) ⟦n ↦ e'⟧ = var (bound v.pred) := by
+  { unfold subs, split_ifs, refl }
+
+lemma subs_bound_eq {n e'} :
+  var (bound n) ⟦n ↦ e'⟧ = e'.gap 0 n := by
+  { unfold subs, split_ifs with hif, { exfalso, exact nat.lt_irrefl _ hif }, refl }
+
+lemma subs_bound_v_lt_n {v n e'} (h : v < n) :
+  var (bound v) ⟦n ↦ e'⟧ = var (bound v) := by
+  { unfold subs, split_ifs with hif₁ hif₂,
+    { exfalso, exact nat.lt_irrefl _ (nat.lt_trans h hif₁) },
+    { rw hif₂ at h, exfalso, exact nat.lt_irrefl _ h },
+    refl }
+
+/- How `gap` interacts with itself. -/
+
+lemma gap_zero (e n) : e ⟦n ↟ 0⟧ = e := by
+{ induction e generalizing n,
+  case sort : s { unfold gap },
+  case var : v { cases v; unfold gap; split_ifs; simp },
+  case app : l r ihl ihr { unfold gap, rw [ihl, ihr] },
+  case lam : t e iht ihe { unfold gap, rw [iht, ihe] },
+  case pi : t₁ t₂ iht₁ iht₂ { unfold gap, rw [iht₁, iht₂] } }
+
+lemma gap_gap_disjoint_ind (e k a b c) : e ⟦k ↟ a⟧ ⟦(a + b + k) ↟ c⟧ = e ⟦(b + k) ↟ c⟧ ⟦k ↟ a⟧ := by
+{ induction e generalizing k,
+  case sort : s { unfold gap },
+  case var : v
+  { cases v, swap, { unfold gap },
+    rcases (lt_or_le v k) with h₁ | h₁,
+    { rw [gap_bound_v_lt_n h₁,
+          gap_bound_v_lt_n (nat.lt_add_left _ _ _ h₁),
+          gap_bound_v_lt_n (nat.lt_add_left _ _ _ h₁),
+          gap_bound_v_lt_n h₁] },
+    rcases (lt_or_le v (b + k)) with h₂ | h₂,
+    { rw [gap_bound_n_le_v h₁, nat.add_comm, nat.add_assoc,
+          gap_bound_v_lt_n (nat.add_lt_add_left h₂ _),
+          gap_bound_v_lt_n h₂,
+          gap_bound_n_le_v h₁, nat.add_comm] },
+    { rw [gap_bound_n_le_v h₁, nat.add_comm, nat.add_assoc,
+          gap_bound_n_le_v (nat.add_le_add_left h₂ _),
+          gap_bound_n_le_v h₂,
+          gap_bound_n_le_v (nat.le_add_right' _ _ _ h₁), nat.add_assoc, nat.add_comm] } },
+  case app : l r ihl ihr { unfold gap, rw [ihl, ihr] },
+  case lam : t e iht ihe { unfold gap, rw [iht, ← nat.add_succ, ihe], refl },
+  case pi : t₁ t₂ iht₁ iht₂ { unfold gap, rw [iht₁, ← nat.add_succ, iht₂], refl } }
+
+lemma gap_gap_disjoint (e a b c) : e ⟦0 ↟ a⟧ ⟦(a + b) ↟ c⟧ = e ⟦b ↟ c⟧ ⟦0 ↟ a⟧ :=
+  gap_gap_disjoint_ind e 0 a b c
+
+lemma gap_gap_overlap_ind (e k a b c) : e ⟦k ↟ (a + b + c)⟧ = e ⟦k ↟ (a + b)⟧ ⟦(k + a) ↟ c⟧ := by
+{ induction e generalizing k,
+  case sort : s { unfold gap },
+  case var : v
+  { cases v, swap, { unfold gap },
+    rcases (lt_or_le v k) with h | h,
+    { rw [gap_bound_v_lt_n h,
+          gap_bound_v_lt_n h,
+          gap_bound_v_lt_n (nat.lt_add_right _ _ _ h)] },
+    { rw [gap_bound_n_le_v h,
+          gap_bound_n_le_v h, ← nat.add_assoc v a b,
+          gap_bound_n_le_v (nat.le_add_right' _ _ _ (nat.add_le_add_right h _)),
+          ← nat.add_assoc, ← nat.add_assoc] } },
+  case app : l r ihl ihr { unfold gap, rw [ihl, ihr] },
+  case lam : t e iht ihe { unfold gap, rw [iht, ihe, nat.succ_add] },
+  case pi : t₁ t₂ iht₁ iht₂ { unfold gap, rw [iht₁, iht₂, nat.succ_add] } }
+
+lemma gap_gap_overlap (e a b c) : e ⟦0 ↟ (a + b + c)⟧ = e ⟦0 ↟ (a + b)⟧ ⟦a ↟ c⟧ :=
+  @eq.subst _ (λ x, e ⟦0 ↟ (a + b + c)⟧ = e ⟦0 ↟ (a + b)⟧ ⟦x ↟ c⟧) _ _
+    (nat.zero_add a) (gap_gap_overlap_ind e 0 a b c)
+
+/- How `gap` and `subs` interact with each other. -/
+
+lemma gap_subs_above_ind (e e' k n m) : e ⟦k ↟ n⟧ ⟦(n + m + k) ↦ e'⟧ = e ⟦(m + k) ↦ e'⟧ ⟦k ↟ n⟧ := by
+{ induction e generalizing k n m,
+  case sort : s { unfold gap subs },
+  case var : v
+  { cases v, swap, { unfold gap subs },
+    rcases (lt_or_le v k) with h₁ | h₁,
+    { rw [gap_bound_v_lt_n h₁,
+          subs_bound_v_lt_n (nat.lt_add_left _ _ _ h₁),
+          subs_bound_v_lt_n (nat.lt_add_left _ _ _ h₁),
+          gap_bound_v_lt_n h₁] },
+    { rw gap_bound_n_le_v h₁,
+      rcases (nat.lt_trichotomy v (m + k)) with h₂ | h₂ | h₂,
+      { rw [subs_bound_v_lt_n h₂, nat.add_comm, nat.add_assoc,
+            subs_bound_v_lt_n (nat.add_lt_add_left h₂ _),
+            gap_bound_n_le_v h₁, nat.add_comm] },
+      { rw [nat.add_comm, nat.add_assoc, h₂,
+            subs_bound_eq,
+            subs_bound_eq, nat.add_comm, nat.add_comm m k,
+            gap_gap_overlap _ _ _ _] },
+      { cases v, { exfalso, exact nat.not_lt_zero _ h₂, },
+        rw [nat.add_comm, nat.add_assoc,
+            subs_bound_n_lt_v (nat.add_lt_add_left h₂ _),
+            subs_bound_n_lt_v h₂, nat.add_succ, nat.pred_succ, nat.pred_succ,
+            gap_bound_n_le_v (nat.le_of_lt_succ (nat.order_aux_2 h₂)), nat.add_comm] } } },
+  case app : l r hl hr { unfold gap subs, rw [hl, hr] },
+  case lam : t e ht he { unfold gap subs, rw [ht, ← nat.add_succ, he], refl },
+  case pi : t₁ t₂ ht₁ ht₂ { unfold gap subs, rw [ht₁, ← nat.add_succ, ht₂], refl } }
+
+lemma gap_subs_above (e e' n m) : e ⟦0 ↟ n⟧ ⟦(n + m) ↦ e'⟧ = e ⟦m ↦ e'⟧ ⟦0 ↟ n⟧ := 
+  gap_subs_above_ind e e' 0 n m
+
+lemma gap_subs_inside_ind (e e' k n m) : e ⟦k ↟ nat.succ (n + m)⟧ ⟦(n + k) ↦ e'⟧ = e ⟦k ↟ (n + m)⟧ := by
+{ induction e generalizing k,
+  case sort : s { unfold gap subs },
+  case var : v
+  { cases v, swap, { unfold gap subs },
+    rcases (lt_or_le v k) with h₁ | h₁,
+    { rw [gap_bound_v_lt_n h₁,
+          gap_bound_v_lt_n h₁,
+          subs_bound_v_lt_n (nat.lt_add_left _ _ _ h₁)] },
+    { rw [gap_bound_n_le_v h₁,
+          gap_bound_n_le_v h₁, nat.add_succ, ← nat.add_assoc, nat.add_comm n k,
+          subs_bound_n_lt_v (nat.lt_succ_of_le (nat.le_add_right' _ _ _ (nat.add_le_add_right h₁ _))),
+          nat.pred_succ] } },
+  case app : l r hl hr { unfold gap subs, rw [hl, hr] },
+  case lam : t e ht he { unfold gap subs, rw [ht, ← nat.add_succ n k, he] },
+  case pi : t₁ t₂ ht₁ ht₂ { unfold gap subs, rw [ht₁, ← nat.add_succ n k, ht₂] } }
+
+lemma gap_subs_inside (e e') {n m} : e ⟦0 ↟ nat.succ (n + m)⟧ ⟦n ↦ e'⟧ = e ⟦0 ↟ (n + m)⟧ :=
+  gap_subs_inside_ind e e' 0 n m
+
+lemma gap_subs_below_ind (e e' k n m) : e ⟦nat.succ (n + k) ↟ m⟧ ⟦k ↦ e' ⟦n ↟ m⟧⟧ = e ⟦k ↦ e'⟧ ⟦(n + k) ↟ m⟧ := by
+{ induction e generalizing k,
+  case sort : s { unfold gap subs },
+  case var : v
+  { cases v, swap, { unfold gap subs },
+    rcases (nat.lt_trichotomy v k) with h₁ | h₁ | h₁,
+    { rw [gap_bound_v_lt_n (nat.lt_succ_of_lt (nat.lt_add_left _ _ _ h₁)),
+          subs_bound_v_lt_n h₁,
+          subs_bound_v_lt_n h₁,
+          gap_bound_v_lt_n (nat.lt_add_left _ _ _ h₁)] },
+    { rw [← h₁,
+          gap_bound_v_lt_n (nat.lt_succ_of_le (nat.le_add_left' _ _ _ (nat.le_refl v))),
+          subs_bound_eq,
+          subs_bound_eq, nat.add_comm,
+          gap_gap_disjoint] },
+    { cases v, { exfalso, exact nat.not_lt_zero _ h₁ },
+      rw subs_bound_n_lt_v h₁,
+      rcases (lt_or_le v (n + k)) with h₂ | h₂,
+      { rw [gap_bound_v_lt_n (nat.succ_lt_succ h₂), nat.pred_succ,
+            subs_bound_n_lt_v h₁,
+            gap_bound_v_lt_n h₂, nat.pred_succ] },
+      { rw [gap_bound_n_le_v (nat.succ_le_succ h₂), nat.pred_succ,
+            subs_bound_n_lt_v (nat.lt_add_right _ _ _ h₁), nat.succ_add,
+            gap_bound_n_le_v h₂, nat.pred_succ] } } },
+  case app : l r ihl ihr { unfold gap subs, rw [ihl, ihr] },
+  case lam : t e iht ihe { unfold gap subs, rw [iht, ← nat.add_succ, ihe],  },
+  case pi : t₁ t₂ iht₁ iht₂ { unfold gap subs, rw [iht₁, ← nat.add_succ, iht₂] } }
+
+lemma gap_subs_below (e e' n m) : e ⟦nat.succ n ↟ m⟧ ⟦0 ↦ e' ⟦n ↟ m⟧⟧ = e ⟦0 ↦ e'⟧ ⟦n ↟ m⟧ :=
+  gap_subs_below_ind e e' 0 n m
+
+/- How `sub` interacts with itself. -/
+
+lemma subs_subs_ind (e e₁ e₂ k n) : e ⟦k ↦ e₁⟧ ⟦(n + k) ↦ e₂⟧ = e ⟦nat.succ (n + k) ↦ e₂⟧ ⟦k ↦ e₁ ⟦n ↦ e₂⟧⟧ := by
+{ induction e generalizing e₁ e₂ k n,
   case sort : s { unfold subs },
   case var : v
-  { unfold subs,
-    cases v with b f,
-    { change b < n.succ at hce,
-      split_ifs with hif; injections; contradiction <|> skip,
-      exact nat.lt_of_le_and_ne (nat.le_of_lt_succ hce) h, },
-    { split_ifs; injections } },
-  case app : l r hl hr { unfold subs, exact c_app (hl hce.1 hce') (hr hce.2 hce') },
-  case lam : t e ht he { unfold subs, exact c_lam (ht hce.1 hce') (he hce.2 (c_weaken₁ hce')) },
-  case pi : t₁ t₂ ht₁ ht₂ { unfold subs, exact c_lam (ht₁ hce.1 hce') (ht₂ hce.2 (c_weaken₁ hce')) } }
+  { cases v, swap, { unfold subs },
+    rcases (nat.lt_trichotomy v k) with h₁ | h₁ | h₁,
+    { rw [subs_bound_v_lt_n h₁,
+          subs_bound_v_lt_n (nat.lt_add_left _ _ _ h₁),
+          subs_bound_v_lt_n (nat.lt_succ_of_lt (nat.lt_add_left _ _ _ h₁)),
+          subs_bound_v_lt_n h₁] },
+    { rw [← h₁,
+          subs_bound_eq,
+          subs_bound_v_lt_n (nat.lt_succ_of_le (nat.le_add_left' _ _ _ (nat.le_refl v))),
+          subs_bound_eq, nat.add_comm,
+          gap_subs_above _ _ _ _] },
+    { cases v, { exfalso, exact nat.not_lt_zero _ h₁ },
+      rcases (nat.lt_trichotomy v (n + k)) with h₂ | h₂ | h₂,
+      { rw [subs_bound_n_lt_v h₁, nat.pred_succ,
+            subs_bound_v_lt_n h₂,
+            subs_bound_v_lt_n (nat.succ_lt_succ h₂),
+            subs_bound_n_lt_v h₁, nat.pred_succ] },
+      { rw [← h₂,
+            subs_bound_n_lt_v h₁, nat.pred_succ,
+            subs_bound_eq,
+            subs_bound_eq, h₂, nat.add_comm,
+            gap_subs_inside] },
+      { rw [subs_bound_n_lt_v h₁, nat.pred_succ,
+            subs_bound_n_lt_v h₂,
+            subs_bound_n_lt_v (nat.succ_lt_succ h₂), nat.pred_succ,
+            subs_bound_n_lt_v (nat.order_aux_2 h₂)] } } },
+  case app : l r ihl ihr { unfold subs, rw [ihl, ihr] },
+  case lam : t e iht ihe { unfold subs, rw iht, simp, exact ihe _ _ _ _ },
+  case pi : t₁ t₂ iht₁ iht₂ { unfold subs, rw iht₁, simp, exact iht₂ _ _ _ _ } }
 
-/-- Substitution at the topmost level 0 makes the term closed. -/
-lemma subs.close₀ {e e'} : closed e 1 → closed e' 0 → closed (subs e 0 e') 0 :=
-  subs.close
+lemma subs_subs (e e₁ e₂ n) : e ⟦0 ↦ e₁⟧ ⟦n ↦ e₂⟧ = e ⟦(nat.succ n) ↦ e₂⟧ ⟦0 ↦ e₁ ⟦n ↦ e₂⟧⟧ :=
+  subs_subs_ind e e₁ e₂ 0 n
 
-/-- `red1 e₁ e₂`: `e₁` reduces to `e₂` by contracting zero or more immediate, disjoint redexes. -/
+/- Uninteresting `size` lemmas to support strong induction on `expr`. -/
+
+lemma size_wf : well_founded (λ e₁ e₂ : expr, size e₁ < size e₂) :=
+  measure_wf size
+
+lemma size_lt_size_app_l {l r} : size l < size (app l r) := by
+{ unfold size, rw [← nat.add_succ], simp }
+
+lemma size_lt_size_app_r {l r} : size r < size (app l r) := by
+{ unfold size, rw [nat.add_comm, ← nat.add_succ], simp }
+
+lemma size_lt_size_lam_l {l r} : size l < size (lam l r) := by
+{ unfold size, rw [← nat.add_succ], simp }
+
+lemma size_lt_size_lam_r {l r} : size r < size (lam l r) := by
+{ unfold size, rw [nat.add_comm, ← nat.add_succ], simp }
+
+lemma size_lt_size_app_lam_e {t e r} : size e < size (app (lam t e) r) :=
+  nat.lt_trans size_lt_size_lam_r size_lt_size_app_l
+
+lemma size_lt_size_pi_l {l r} : size l < size (pi l r) := by
+{ unfold size, rw [← nat.add_succ], simp }
+
+lemma size_lt_size_pi_r {l r} : size r < size (pi l r) := by
+{ unfold size, rw [nat.add_comm, ← nat.add_succ], simp }
+
+end
+end expr
+open expr
+
+/- Main part. -/
+
+/-- The "one-step reduction" relation `red1 e₁ e₂`: "`e₁` reduces to `e₂` by contracting zero or more immediate redexes."
+    See: https://archive-pml.github.io/martin-lof/pdfs/An-Intuitionistic-Theory-of-Types-1972.pdf -/
 inductive red1 : expr → expr → Prop
-| r1_beta {t e r}         : red1 (app (lam t e) r) (e.subs 0 r)
-| r1_sort (s)             :                             red1 (sort s) (sort s)
-| r1_var  (v)             :                             red1 (var v) (var v)
+| r1_beta {t e e' r r'}   : red1 e e' → red1 r r' →     red1 (app (lam t e) r) (e'⟦0 ↦ r'⟧)
+| r1_sort {s}             :                             red1 (sort s) (sort s)
+| r1_var  {v}             :                             red1 (var v) (var v)
 | r1_app  {l l' r r'}     : red1 l l' → red1 r r' →     red1 (app l r) (app l' r')
 | r1_lam  {t t' e e'}     : red1 t t' → red1 e e' →     red1 (lam t e) (lam t' e')
 | r1_pi   {t₁ t₁' t₂ t₂'} : red1 t₁ t₁' → red1 t₂ t₂' → red1 (pi t₁ t₂) (pi t₁' t₂')
@@ -78,47 +298,78 @@ open red1
 
 local notation e ` ~>₁ ` e' := red1 e e'
 
-lemma red1.refl (e : expr) : e ~>₁ e :=
+lemma red1.refl {e : expr} : e ~>₁ e :=
   @expr.rec_on (λ e, e ~>₁ e) e
-    r1_sort r1_var (λ _ _, r1_app) (λ _ _, r1_lam) (λ _ _, r1_pi)
+    (λ _, r1_sort) (λ _, r1_var) (λ _ _, r1_app) (λ _ _, r1_lam) (λ _ _, r1_pi)
 
-lemma red1.of_red1_left_rep
-  {e e' e₁ : expr}
-  (hce : closed e 0) (hce' : closed e' 0) (hce₁ : closed e₁ 0)
-  (h : e ~>₁ e') :
-  e⟦e₁/$⟧ ~>₁ e'⟦e₁/$⟧ := by
-{ induction h,
-  case r1_beta : t e r
-  {  },
-  case r1_sort : h
-  { admit },
-  case r1_var : h
-  { admit },
-  case r1_app : h_l h_l' h_r h_r' h_ᾰ h_ᾰ_1 h_ih_ᾰ h_ih_ᾰ_1
-  { admit },
-  case r1_lam : h_t h_t' h_e h_e' h_ᾰ h_ᾰ_1 h_ih_ᾰ h_ih_ᾰ_1
-  { admit },
-  case r1_pi : h_t₁ h_t₁' h_t₂ h_t₂' h_ᾰ h_ᾰ_1 h_ih_ᾰ h_ih_ᾰ_1
-  { admit }}
+lemma red1.red1_gap_ind (n e e' k) (h : e ~>₁ e') : e ⟦k ↟ n⟧ ~>₁ e' ⟦k ↟ n⟧ := by
+{ -- Strong induction on `e` generalising `e' k h`.
+  revert_after e, apply size_wf.induction e, intros e ih,
+  cases e,
+  case sort : s { intros, cases h, unfold gap, exact red1.refl },
+  case var : v { intros, cases h, cases v; split_ifs <|> skip; exact red1.refl },
+  case app : l r
+  { intros,
+    cases h,
+    case r1_beta : t e e' r r' he hr
+    { unfold gap, rw ← gap_subs_below,
+      refine r1_beta (ih e _ _ _ _) (ih r _ _ _ _), assumption',
+      exacts [size_lt_size_app_lam_e, size_lt_size_app_r] },
+    case r1_app : l l' r r' hl hr
+    { unfold gap, refine r1_app (ih l _ _ _ _) (ih r _ _ _ _), assumption',
+      exacts [size_lt_size_app_l, size_lt_size_app_r] } },
+  case lam : t e
+  { intros, cases h, unfold gap,
+    refine r1_lam (ih t _ _ _ _) (ih e _ _ _ _), assumption',
+    exacts [size_lt_size_lam_l, size_lt_size_lam_r] },
+  case pi : t₁ t₂
+  { intros, cases h, unfold gap,
+    refine r1_pi (ih t₁ _ _ _ _) (ih t₂ _ _ _ _), assumption',
+    exacts [size_lt_size_pi_l, size_lt_size_pi_r] } }
 
-lemma red1.confluent {e e₁ e₂ : expr} (h₁ : e ~>₁ e₁) (h₂ : e ~>₁ e₂) :
-  ∃ e', (e₁ ~>₁ e') ∧ (e₂ ~>₁ e') := by
-{ induction e generalizing e₁ e₂,
-  case sort : s { cases h₁, cases h₂, use (sort s), exact ⟨r1_sort s, r1_sort s⟩, },
-  case var : v { cases h₁, cases h₂, use (var v), exact ⟨r1_var v, r1_var v⟩ },
-  case app : l r ihl ihr
-  { cases h₁,
-    case r1_app : l l₁ r r₁ hl₁ hr₁
-    { cases h₂,
-      case r1_beta : t e r
-      { rcases hl₁ with _ | _ | _ | _ | @⟨t, t', e, e', ht, he⟩ | _,
-        use e'.subs 0 r,
-         },
-      case r1_app : l l₂ r r₂ hl₂ hr₂
-      { cases ihl hl₁ hl₂ with el hel,
-        cases ihr hr₁ hr₂ with er her,
-        use (app el er), exact ⟨r1_app hel.1 her.1, r1_app hel.2 her.2⟩ }}
-  }
+lemma red1.red1_gap (n) {e e'} (h : e ~>₁ e') : e ⟦0 ↟ n⟧ ~>₁ e' ⟦0 ↟ n⟧ :=
+  red1.red1_gap_ind n e e' 0 h
+
+lemma red1.red1_subs_ind {l l'} (hl : l ~>₁ l') {r r'} (hr : r ~>₁ r') (k) : l ⟦k ↦ r⟧ ~>₁ l' ⟦k ↦ r'⟧ := by
+{ revert_all, intros l₀ l₀' hl₀ r₀ r₀' hr₀ k,
+  -- Strong induction on `l₀` generalising `l₀' hl₀ r₀ r₀' hr₀ k`.
+  revert_after l₀, apply size_wf.induction l₀, intros l₀ ih,
+  cases l₀,
+  case sort : s { intros, cases hl₀, unfold subs, exact r1_sort },
+  case var : v
+  { intros, cases v; cases hl₀; unfold subs, swap, apply r1_var,
+    split_ifs; exact red1.refl <|> skip,
+    exact red1.red1_gap k hr₀ },
+  case app : l r
+  { intros,
+    cases hl₀,
+    case r1_beta : t e e' r r' he hr
+    { unfold subs, rw subs_subs,
+      refine r1_beta (ih e _ _ _ _) (ih r _ _ _ _), assumption',
+      exacts [size_lt_size_app_lam_e, size_lt_size_app_r] },
+    case r1_app : l l' r r' hl hr
+    { unfold subs,
+      refine r1_app (ih l _ _ _ _) (ih r _ _ _ _), assumption',
+      exacts [size_lt_size_app_l, size_lt_size_app_r] } },
+  case lam : t e
+  { intros, cases hl₀, unfold subs,
+    refine r1_lam (ih t _ _ _ _) (ih e _ _ _ _), assumption',
+    exacts [size_lt_size_lam_l, size_lt_size_lam_r] },
+  case pi : t₁ t₂
+  { intros, cases hl₀, unfold subs,
+    refine r1_pi (ih t₁ _ _ _ _) (ih t₂ _ _ _ _), assumption',
+    exacts [size_lt_size_pi_l, size_lt_size_pi_r] } }
+
+lemma red1.confluent {a b c : expr} (hb : a ~>₁ b) (hc : a ~>₁ c) :
+  ∃ d, (b ~>₁ d) ∧ (c ~>₁ d) := by
+{ -- Strong induction on `a` generalising `b c hb hc`.
+  revert_after a, apply size_wf.induction a, intros a ih,
+  cases a,
+  case sort : s { intros, cases hb, cases hc, use (sort s), exact ⟨r1_sort, r1_sort⟩, },
+  case var : v { intros, cases hb, cases hc, use (var v), exact ⟨r1_var, r1_var⟩ },
+  case app : l r { sorry },
+  case lam : l r { sorry },
+  case pi : l r { sorry }
 }
 
 end
